wip

crypto/bignum/x25519/Hacl.EC.AddAndDouble.fst
@@ -6,36 +6,248 @@ open FStar.Buffer
 open Hacl.Bignum.Constants
 open Hacl.Bignum.Parameters
 open Hacl.Bignum
-open Hacl.EC.Point
+open Hacl.Bignum.Fsquare
 open Hacl.Spec.EC.AddAndDouble2
 
 
-let all_disjoint ppx ppz ppqx ppqz px pz pqx pqz qx qz =
+#set-options "--initial_fuel 0 --max_fuel 0"
+
+let all_disjoint (ppx:felem) (ppz:felem) (ppqx:felem) (ppqz:felem)
+                 (px:felem) (pz:felem) (pqx:felem) (pqz:felem) (qx:felem) : GTot Type0 =
   disjoint ppx ppz /\ disjoint ppx ppqx /\ disjoint ppx ppqz /\ disjoint ppx px /\ disjoint ppx pz
-  /\ disjoint ppx pqx /\ disjoint ppx pqz /\ disjoint ppx qx /\ disjoint ppx qz
+  /\ disjoint ppx pqx /\ disjoint ppx pqz /\ disjoint ppx qx
   /\ disjoint ppz ppqx /\ disjoint ppz ppqz /\ disjoint ppz px /\ disjoint ppz pz
-  /\ disjoint ppz pqx /\ disjoint ppz pqz /\ disjoint ppz qx /\ disjoint ppz qz
+  /\ disjoint ppz pqx /\ disjoint ppz pqz /\ disjoint ppz qx
   /\ disjoint ppqx ppqz /\ disjoint ppqx px /\ disjoint ppqx pz
-  /\ disjoint ppqx pqx /\ disjoint ppqx pqz /\ disjoint ppqx qx /\ disjoint ppqx qz
+  /\ disjoint ppqx pqx /\ disjoint ppqx pqz /\ disjoint ppqx qx
   /\ disjoint ppqz px /\ disjoint ppqz pz
-  /\ disjoint ppqz pqx /\ disjoint ppqz pqz /\ disjoint ppqz qx /\ disjoint ppqz qz
-  /\ disjoint px pz /\ disjoint px pqx /\ disjoint px pqz /\ disjoint px qx /\ disjoint px qz
-  /\ disjoint pz pqx /\ disjoint pz pqz /\ disjoint pz qx /\ disjoint pz qz
-  /\ disjoint pqx pqz /\ disjoint pqx qx /\ disjoint pqx qz
-  /\ disjoint pqz qx /\ disjoint pqz qz
-  /\ disjoint qx qz
+  /\ disjoint ppqz pqx /\ disjoint ppqz pqz /\ disjoint ppqz qx
+  /\ disjoint px pz /\ disjoint px pqx /\ disjoint px pqz /\ disjoint px qx
+  /\ disjoint pz pqx /\ disjoint pz pqz /\ disjoint pz qx
+  /\ disjoint pqx pqz /\ disjoint pqx qx
+  /\ disjoint pqz qx
 
 
-val fmonty:
+inline_for_extraction let red_52 s = Hacl.Spec.EC.AddAndDouble.red_52 s
+
+
+(* val fmonty_1: *)
+(*   tmp:FStar.Buffer.buffer Hacl.UInt64.t{length tmp = 40} -> *)
+(*   ppx:felem -> ppz:felem -> ppqx:felem -> ppqz:felem -> *)
+(*   px:felem -> pz:felem -> pqx:felem -> pqz:felem -> *)
+(*   qx:felem -> *)
+(*   Stack unit *)
+(*     (requires (fun h -> live h tmp *)
+(*       /\ live h ppx /\ live h ppz /\ live h ppqx /\ live h ppqz *)
+(*       /\ live h px /\ live h pz /\ live h pqx /\ live h pqz *)
+(*       /\ live h qx *)
+(*       /\ red_52 (as_seq h px) /\ red_52 (as_seq h pz) /\ red_52 (as_seq h pqx) /\ red_52 (as_seq h pqz) *)
+(*       /\ red_52 (as_seq h qx) *)
+(*       /\ all_disjoint ppx ppz ppqx ppqz px pz pqx pqz qx *)
+(*       /\ disjoint tmp ppx /\ disjoint tmp ppz /\ disjoint tmp ppqx /\ disjoint tmp ppqz *)
+(*       /\ disjoint tmp px /\ disjoint tmp pz /\ disjoint tmp pqx /\ disjoint tmp pqz *)
+(*       /\ disjoint tmp qx *)
+(*       )) *)
+(*     (ensures (fun h0 _ h1 -> *)
+(*       live h0 ppx /\ live h0 ppz /\ live h0 ppqx /\ live h0 ppqz *)
+(*       /\ live h0 px /\ live h0 pz /\ live h0 pqx /\ live h0 pqz *)
+(*       /\ live h0 qx /\ live h0 qz *)
+(*       /\ live h1 ppx /\ live h1 ppz /\ live h1 ppqx /\ live h1 ppqz *)
+(*       /\ red_52 (as_seq h0 px) /\ red_52 (as_seq h0 pz) /\ red_52 (as_seq h0 pqx) /\ red_52 (as_seq h0 pqz) *)
+(*       /\ red_52 (as_seq h0 qx) /\ red_52 (as_seq h0 qz) *)
+(*       /\ all_disjoint ppx ppz ppqx ppqz px pz pqx pqz qx qz *)
+(*       /\ (as_seq h1 ppx, as_seq h1 ppz, as_seq h1 ppqx, as_seq h1 ppqz) == *)
+(*           fmonty_tot (as_seq h0 px) (as_seq h0 pz) (as_seq h0 pqx) (as_seq h0 pqz) (as_seq h0 qx) (as_seq h0 qz) *)
+(*     )) *)
+(* #set-options "--initial_fuel 0 --max_fuel 0 --z3rlimit 100" *)
+(* let fmonty_1 buf x2 z2 x3 z3 x z xprime zprime qx = *)
+(*   let origx      = Buffer.sub buf 0ul  5ul in *)
+(*   let origxprime = Buffer.sub buf 5ul  5ul in *)
+(*   let zzz        = Buffer.sub buf 10ul 5ul in *)
+(*   let xx         = Buffer.sub buf 15ul 5ul in *)
+(*   let zz         = Buffer.sub buf 20ul 5ul in *)
+(*   let xxprime    = Buffer.sub buf 25ul 5ul in *)
+(*   let zzprime    = Buffer.sub buf 30ul 5ul in *)
+(*   let zzzprime   = Buffer.sub buf 35ul 5ul in *)
+(*   let h0 = ST.get() in *)
+(*   blit x 0ul origx 0ul 5ul; *)
+(*   let h1 = ST.get() in *)
+(*   Hacl.Spec.Bignum.Fmul.lemma_whole_slice (as_seq h0 x); *)
+(*   Hacl.Spec.Bignum.Fmul.lemma_whole_slice (as_seq h1 origx); *)
+(*   Hacl.Spec.EC.AddAndDouble.fsum_52_is_53 (as_seq h1 x) (as_seq h1 z); *)
+(*   fsum x z; // x < x + z *)
+(*   let h2 = ST.get() in *)
+(*   Hacl.Spec.EC.AddAndDouble.lemma_fdifference_unrolled' (as_seq h2 z) (as_seq h2 origx); *)
+(*   fdifference z origx; // z <- 8p + x - z *)
+(*   let h3 = ST.get() in *)
+(*   blit xprime 0ul origxprime 0ul 5ul; *)
+(*   let h4 = ST.get() in *)
+(*   Hacl.Spec.Bignum.Fmul.lemma_whole_slice (as_seq h3 xprime); *)
+(*   Hacl.Spec.Bignum.Fmul.lemma_whole_slice (as_seq h4 origxprime); *)
+(*   Hacl.Spec.EC.AddAndDouble.fsum_52_is_53 (as_seq h4 xprime) (as_seq h4 zprime); *)
+(*   fsum xprime zprime; // xprime <- xprime + zprime *)
+(*   let h5 = ST.get() in *)
+(*   Hacl.Spec.EC.AddAndDouble.lemma_fdifference_unrolled' (as_seq h5 zprime) (as_seq h5 origxprime); *)
+(*   fdifference zprime origxprime; // zprime <- 8p + xprime - zprime *)
+(*   let h6 = ST.get() in *)
+(*   Hacl.Spec.EC.AddAndDouble.fmul_53_55_is_fine (as_seq h6 xprime) (as_seq h6 z); *)
+(*   fmul xxprime xprime z; // xxprime <- sum * sub *)
+(*   let h7 = ST.get() in *)
+(*   Hacl.Spec.EC.AddAndDouble.fmul_53_55_is_fine (as_seq h7 x) (as_seq h7 zprime); *)
+(*   fmul zzprime x zprime; // zzprime <- sum * sub *)
+(*   () *)
+
+
+(* val fmonty_1: *)
+(*   tmp:FStar.Buffer.buffer Hacl.UInt64.t{length tmp = 40} -> *)
+(*   ppx:felem -> ppz:felem -> ppqx:felem -> ppqz:felem -> *)
+(*   px:felem -> pz:felem -> pqx:felem -> pqz:felem -> *)
+(*   qx:felem -> *)
+(*   Stack unit *)
+(*     (requires (fun h -> *)
+(*       live h ppx /\ live h ppz /\ live h ppqx /\ live h ppqz *)
+(*       /\ live h px /\ live h pz /\ live h pqx /\ live h pqz *)
+(*       /\ live h qx /\ live h tmp *)
+(*       /\ red_52 (as_seq h px) /\ red_52 (as_seq h pz) /\ red_52 (as_seq h pqx) /\ red_52 (as_seq h pqz) *)
+(*       /\ red_52 (as_seq h qx) *)
+(*       /\ all_disjoint ppx ppz ppqx ppqz px pz pqx pqz qx *)
+(*       /\ disjoint tmp ppx /\ disjoint tmp ppz /\ disjoint tmp ppqx /\ disjoint tmp ppqz *)
+(*       /\ disjoint tmp px /\ disjoint tmp pz /\ disjoint tmp pqx /\ disjoint tmp pqz *)
+(*       /\ disjoint tmp qx *)
+(*       )) *)
+(*     (ensures (fun h0 _ h1 -> true)) *)
+(* let fmonty_2 buf ppx ppz ppqx ppqz p pz pqx pqz qx = *)
+(*   let h8 = ST.get() in *)
+(*   blit xxprime 0ul origxprime 0ul 5ul; *)
+(*   let h9 = ST.get() in *)
+(*   Hacl.Spec.Bignum.Fmul.lemma_whole_slice (as_seq h8 xxprime); *)
+(*   Hacl.Spec.Bignum.Fmul.lemma_whole_slice (as_seq h9 origxprime); *)
+(*   Hacl.Spec.EC.AddAndDouble.fsum_52_is_53 (as_seq h9 xxprime) (as_seq h9 zzprime); *)
+(*   fsum xxprime zzprime; // xxprime <- sum *)
+(*   let h10 = ST.get() in *)
+(*   Hacl.Spec.EC.AddAndDouble.lemma_fdifference_unrolled' (as_seq h10 zzprime) (as_seq h10 origxprime); *)
+(*   fdifference zzprime origxprime; // zzprime <- sub *)
+(*   admit() *)
+(*   let h11 = ST.get() in *)
+(*   fsquare_times x3 xxprime 1ul; // sum sum *)
+(*   let h12 = ST.get() in *)
+(*   fsquare_times zzzprime zzprime 1ul; // sub sub *)
+(*   let h13 = ST.get() in *)
+(*   fmul z3 zzzprime qx; *)
+(*   let h14 = ST.get() in *)
+(*   fsquare_times xx x 1ul; // sum red *)
+(*   let h15 = ST.get() in *)
+(*   fsquare_times zz z 1ul; // red sub *)
+(*   let h16 = ST.get() in *)
+(*   fmul x2 xx zz; // red red *)
+(*   let h17 = ST.get() in *)
+(*   fdifference zz xx; // red red *)
+(*   let h18 = ST.get() in *)
+(*   fscalar zzz zz (uint64_to_limb Hacl.Bignum.Constants.a24); *)
+(*   let h19 = ST.get() in *)
+(*   fsum zzz xx; // red red *)
+(*   let h20 = ST.get() in *)
+(*   fmul z2 zz zzz; *)
+(*   pop_frame() *)
+
+
+(* ********************************************************************************* *)
+(* ********************************************************************************* *)
+
+
+val fmonty_:
   ppx:felem -> ppz:felem -> ppqx:felem -> ppqz:felem ->
   px:felem -> pz:felem -> pqx:felem -> pqz:felem ->
-  qx:felem -> qz:felem -> Stack unit
-    (requires (fun h -> live h ppx /\ live h ppz /\ live h ppqx /\ live h ppqz
+  qx:felem -> Stack unit
+    (requires (fun h ->
+      live h ppx /\ live h ppz /\ live h ppqx /\ live h ppqz
       /\ live h px /\ live h pz /\ live h pqx /\ live h pqz
-      /\ all_disjoint ppx ppz ppqx ppqz px pz pqx pqz qx qz))
-    (ensures (fun h -> live h ppx /\ live h ppz /\ live h ppqx /\ live h ppqz
-      /\ live h px /\ live h pz /\ live h pqx /\ live h pqz
-      /\ as_seq
+      /\ live h qx
+      /\ red_52 (as_seq h px) /\ red_52 (as_seq h pz) /\ red_52 (as_seq h pqx) /\ red_52 (as_seq h pqz)
+      /\ red_52 (as_seq h qx)
+      /\ all_disjoint ppx ppz ppqx ppqz px pz pqx pqz qx))
+    (ensures (fun h0 _ h1 ->
+      live h0 ppx /\ live h0 ppz /\ live h0 ppqx /\ live h0 ppqz
+      /\ live h0 px /\ live h0 pz /\ live h0 pqx /\ live h0 pqz
+      /\ live h0 qx
+      /\ live h1 ppx /\ live h1 ppz /\ live h1 ppqx /\ live h1 ppqz
+      /\ red_52 (as_seq h0 px) /\ red_52 (as_seq h0 pz) /\ red_52 (as_seq h0 pqx) /\ red_52 (as_seq h0 pqz)
+      /\ red_52 (as_seq h0 qx)
+      /\ all_disjoint ppx ppz ppqx ppqz px pz pqx pqz qx
+      /\ (as_seq h1 ppx, as_seq h1 ppz, as_seq h1 ppqx, as_seq h1 ppqz) ==
+          fmonty_tot (as_seq h0 px) (as_seq h0 pz) (as_seq h0 pqx) (as_seq h0 pqz) (as_seq h0 qx)
+    ))
+#set-options "--initial_fuel 0 --max_fuel 0 --z3rlimit 100"
+let fmonty_ x2 z2 x3 z3 x z xprime zprime qx qmqpz =
+  push_frame();
+  let buf = create limb_zero 40ul in
+  let origx      = Buffer.sub buf 0ul  5ul in
+  let origxprime = Buffer.sub buf 5ul  5ul in
+  let zzz        = Buffer.sub buf 10ul 5ul in
+  let xx         = Buffer.sub buf 15ul 5ul in
+  let zz         = Buffer.sub buf 20ul 5ul in
+  let xxprime    = Buffer.sub buf 25ul 5ul in
+  let zzprime    = Buffer.sub buf 30ul 5ul in
+  let zzzprime   = Buffer.sub buf 35ul 5ul in
+  let h0 = ST.get() in
+  blit x 0ul origx 0ul 5ul;
+  let h1 = ST.get() in
+  Hacl.Spec.Bignum.Fmul.lemma_whole_slice (as_seq h0 x);
+  Hacl.Spec.Bignum.Fmul.lemma_whole_slice (as_seq h1 origx);
+  Hacl.Spec.EC.AddAndDouble.fsum_52_is_53 (as_seq h1 x) (as_seq h1 z);
+  fsum x z; // x < x + z
+  let h2 = ST.get() in
+  Hacl.Spec.EC.AddAndDouble.lemma_fdifference_unrolled' (as_seq h2 z) (as_seq h2 origx);
+  fdifference z origx; // z <- 8p + x - z
+  let h3 = ST.get() in
+  blit xprime 0ul origxprime 0ul 5ul;
+  let h4 = ST.get() in
+  Hacl.Spec.Bignum.Fmul.lemma_whole_slice (as_seq h3 xprime);
+  Hacl.Spec.Bignum.Fmul.lemma_whole_slice (as_seq h4 origxprime);
+  Hacl.Spec.EC.AddAndDouble.fsum_52_is_53 (as_seq h4 xprime) (as_seq h4 zprime);
+  fsum xprime zprime; // xprime <- xprime + zprime
+  let h5 = ST.get() in
+  Hacl.Spec.EC.AddAndDouble.lemma_fdifference_unrolled' (as_seq h5 zprime) (as_seq h5 origxprime);
+  fdifference zprime origxprime; // zprime <- 8p + xprime - zprime
+  let h6 = ST.get() in
+  Hacl.Spec.EC.AddAndDouble.fmul_53_55_is_fine (as_seq h6 xprime) (as_seq h6 z);
+  fmul xxprime xprime z; // xxprime <- sum * sub
+  let h7 = ST.get() in
+  Hacl.Spec.EC.AddAndDouble.fmul_53_55_is_fine (as_seq h7 x) (as_seq h7 zprime);
+  fmul zzprime x zprime; // zzprime <- sum * sub
+  let h8 = ST.get() in
+  blit xxprime 0ul origxprime 0ul 5ul;
+  let h9 = ST.get() in
+  Hacl.Spec.Bignum.Fmul.lemma_whole_slice (as_seq h8 xxprime);
+  Hacl.Spec.Bignum.Fmul.lemma_whole_slice (as_seq h9 origxprime);
+  Hacl.Spec.EC.AddAndDouble.fsum_52_is_53 (as_seq h9 xxprime) (as_seq h9 zzprime);
+  fsum xxprime zzprime; // xxprime <- sum
+  let h10 = ST.get() in
+  Hacl.Spec.EC.AddAndDouble.lemma_fdifference_unrolled' (as_seq h10 zzprime) (as_seq h10 origxprime);
+  fdifference zzprime origxprime; // zzprime <- sub
+  admit()
+  let h11 = ST.get() in
+  fsquare_times x3 xxprime 1ul; // sum sum
+  let h12 = ST.get() in
+  fsquare_times zzzprime zzprime 1ul; // sub sub
+  let h13 = ST.get() in
+  fmul z3 zzzprime qx;
+  let h14 = ST.get() in
+  fsquare_times xx x 1ul; // sum red
+  let h15 = ST.get() in
+  fsquare_times zz z 1ul; // red sub
+  let h16 = ST.get() in
+  fmul x2 xx zz; // red red
+  let h17 = ST.get() in
+  fdifference zz xx; // red red
+  let h18 = ST.get() in
+  fscalar zzz zz (uint64_to_limb Hacl.Bignum.Constants.a24);
+  let h19 = ST.get() in
+  fsum zzz xx; // red red
+  let h20 = ST.get() in
+  fmul z2 zz zzz;
+  pop_frame()
+
 
 val fmonty:
   pp:point ->
@@ -78,10 +290,10 @@ let fmonty pp ppq p pq qmqp =
   fsum xxprime zzprime; // xxprime <- sum
   fdifference zzprime origxprime; // zzprime <- sub
   fsquare_times x3 xxprime 1ul; // sum sum
-  fsquare_times zzzprime zzprime 1ul; // sub sub 
+  fsquare_times zzzprime zzprime 1ul; // sub sub
   fmul z3 zzzprime qx;
   fsquare_times xx x 1ul; // sum red
-  fsquare_times zz z 1ul; // red sub 
+  fsquare_times zz z 1ul; // red sub
   fmul x2 xx zz; // red red
   fdifference zz xx; // red red
   fscalar zzz zz (uint64_to_limb Hacl.Bignum.Constants.a24);
