crypto/bignum/poly1305/Hacl.Bignum.Modulo.fst
@@ -11,29 +11,6 @@ open Hacl.Bignum.Limb
 open Hacl.Spec.Bignum.Modulo
 
 
-let add_zero b = admit()
-  (* let b0 = b.(0ul) in *)
-  (* let b1 = b.(1ul) in *)
-  (* let b2 = b.(2ul) in *)
-  (* let b3 = b.(3ul) in *)
-  (* let b4 = b.(4ul) in *)
-  (* b.(0ul) <- b0 +^ two54m152; *)
-  (* b.(1ul) <- b1 +^ two54m8; *)
-  (* b.(2ul) <- b2 +^ two54m8; *)
-  (* b.(3ul) <- b3 +^ two54m8; *)
-  (* b.(4ul) <- b4 +^ two54m8 *)
-
-let carry_top b = admit()
-  (* let b4 = b.(4ul) in *)
-  (* let b0 = b.(0ul) in *)
-  (* let mask = (limb_one <<^ climb_size) -^ limb_one in *)
-  (* let nineteen = (limb_one <<^ 4ul) +^ (limb_one <<^ 1ul) +^ limb_one in *)
-  (* let b4' = b4 &^ mask in *)
-  (* let b0' = b0 +^ (nineteen *^ (b4 >>^ climb_size)) in *)
-  (* b.(4ul) <- b4'; *)
-  (* b.(0ul) <- b0' *)
-
-
 let reduce b =
   let b0 = b.(0ul) in
   b.(0ul) <- (five <<^ 2ul) *^ b0
