crypto/bignum/x25519/Hacl.Spec.EC.AddAndDouble2.fst
@@ -1,0 +1,45 @@
+module Hacl.Spec.EC.AddAndDouble2
+
+open Hacl.Bignum.Constants
+open Hacl.Bignum.Parameters
+open Hacl.Spec.Bignum
+open Hacl.Spec.Bignum.Fsquare
+open Hacl.Spec.Bignum.Fmul
+open Hacl.Spec.EC.AddAndDouble
+
+
+#set-options "--initial_fuel 0 --max_fuel 0"
+
+val fmonty_tot:
+  px:seqelem{red_52 px} -> pz:seqelem{red_52 pz} ->
+  pqx:seqelem{red_52 pqx} -> pqz:seqelem{red_52 pqz} ->
+  qx:seqelem{red_52 qx} ->
+  Tot (seqelem * seqelem * seqelem * seqelem)
+let fmonty_tot px pz pqx pqz qx =
+  fsum_52_is_53 px pz;
+  let px' = fsum_tot px pz in
+  lemma_fdifference_unrolled' pz px;
+  let pz' = fdifference_tot pz px in
+  fsum_52_is_53 pqx pqz;
+  let pqx' = fsum_tot pqx pqz in
+  lemma_fdifference_unrolled' pqz pqx;
+  let pqz' = fdifference_tot pqz pqx in
+  fmul_53_55_is_fine pqx' pz';
+  let xxprime = fmul_tot pqx' pz' in
+  fmul_53_55_is_fine px' pqz';
+  let zzprime = fmul_tot px' pqz' in
+  fsum_52_is_53 xxprime zzprime;
+  let xxprime' = fsum_tot xxprime zzprime in
+  lemma_fdifference_unrolled' zzprime pqx;
+  let zzprime' = fdifference_tot zzprime pqx in
+  let x3 = fsquare_times_tot xxprime' 1 in
+  let zzzprime = fsquare_times_tot zzprime' 1 in
+  let z3 = fmul_tot zzzprime qx in
+  let xx = fsquare_times_tot px' 1 in
+  let zz = fsquare_times_tot pz' 1 in
+  let x2 = fmul_tot xx zz in
+  let zz' = fdifference_tot zz xx in
+  let zzz = fscalar_tot zz (uint64_to_limb Hacl.Bignum.Constants.a24) in
+  let zzz' = fsum_tot zzz xx in
+  let z2 = fsum_tot zz' zzz' in
+  (x2, z2, x3, z3)
